compiler/backend/word_instScript.sml
@@ -28,14 +28,14 @@ val num_exp_def = Define `
     5 ..
 *)
 
-val flatten_exp_def = tDefine "flatten_exp" ` 
-  (flatten_exp (Op Sub exps) = Op Sub (MAP flatten_exp exps)) ∧ 
-  (flatten_exp (Op And []) = Const (~0w)) ∧ (*I guess this should never occur..*) 
-  (flatten_exp (Op op []) = Const (0w)) ∧ (*I guess this should never occur..*) 
+val flatten_exp_def = tDefine "flatten_exp" `
+  (flatten_exp (Op Sub exps) = Op Sub (MAP flatten_exp exps)) ∧
+  (flatten_exp (Op And []) = Const (~0w)) ∧ (*I guess this should never occur..*)
+  (flatten_exp (Op op []) = Const (0w)) ∧ (*I guess this should never occur..*)
   (flatten_exp (Op op [x]) = flatten_exp x) ∧
   (flatten_exp (Op op (x::xs)) = Op op [flatten_exp x;flatten_exp (Op op xs)]) ∧
-  (flatten_exp (Load exp) = Load (flatten_exp exp)) ∧ 
-  (flatten_exp (Shift shift exp nexp) = Shift shift (flatten_exp exp) nexp) ∧ 
+  (flatten_exp (Load exp) = Load (flatten_exp exp)) ∧
+  (flatten_exp (Shift shift exp nexp) = Shift shift (flatten_exp exp) nexp) ∧
   (flatten_exp exp = exp)`
   (WF_REL_TAC `measure (exp_size ARB)`
    \\ REPEAT STRIP_TAC \\ IMP_RES_TAC MEM_IMP_exp_size
@@ -54,7 +54,7 @@ val flatten_exp_def = tDefine "flatten_exp" `
   Store exp var
 
   Next, perform instruction selection assuming input is binary branching
-  Each step takes tar and temp where we are allowed to store temporaries 
+  Each step takes tar and temp where we are allowed to store temporaries
   in temp and the value of the whole expression must be saved in tar
 *)
 val inst_select_exp_def = tDefine "inst_select_exp" `
@@ -62,8 +62,8 @@ val inst_select_exp_def = tDefine "inst_select_exp" `
   (*
   (inst_select_exp (c:'a asm_config) (tar:num) (temp:num) (Load (Op Add [Const w;exp])) =
     let prog = inst_select_exp c temp temp exp in
-      if addr_offset_ok w c 
-      then 
+      if addr_offset_ok w c
+      then
         Seq prog (Inst (Mem Load tar (Addr temp w)))
       else if c.valid_imm (INL Add) w
       then
@@ -75,17 +75,17 @@ val inst_select_exp_def = tDefine "inst_select_exp" `
         let prog'' = Inst (Arith (Binop Add temp temp (Reg (temp+1)))) in
         let prog''' = Inst (Mem Load tar (Addr temp 0w)) in
         Seq prog (Seq prog' (Seq prog'' prog'''))) ∧*)
-   (inst_select_exp (c:'a asm_config) tar temp (Load exp:'a exp) = 
+   (inst_select_exp (c:'a asm_config) tar temp (Load exp:'a exp) =
     let prog = inst_select_exp c temp temp exp in
-    Seq prog (Inst (Mem Load tar (Addr temp (0w))))) ∧ 
+    Seq prog (Inst (Mem Load tar (Addr temp (0w))))) ∧
   (inst_select_exp c (tar:num) (temp:num) (Const w) = (Inst (Const tar w))) ∧
   (inst_select_exp c (tar:num) (temp:num) (Var v) =
     Move 0 [tar,v]) ∧
-  (inst_select_exp c tar temp (Lookup store_name) = 
-    Get tar store_name) ∧ 
+  (inst_select_exp c tar temp (Lookup store_name) =
+    Get tar store_name) ∧
   (*All ops are binary branching*)
   (*
-  (inst_select_exp c tar temp (Op op [Const w;e2]) = 
+  (inst_select_exp c tar temp (Op op [Const w;e2]) =
     let p2 = inst_select_exp c (temp+1) (temp+1) e2 in
     if c.valid_imm (INL op) w then
       Seq p2 (Inst (Arith (Binop op tar temp (Imm w))))
@@ -95,12 +95,17 @@ val inst_select_exp_def = tDefine "inst_select_exp" `
   (inst_select_exp c tar temp (Op op [e1;e2]) =
     let p1 = inst_select_exp c temp temp e1 in
     let p2 = inst_select_exp c (temp+1) (temp+1) e2 in
-    Seq p1 (Seq p2 (Inst (Arith (Binop op tar temp (Reg (temp+1))))))) ∧ 
+    Seq p1 (Seq p2 (Inst (Arith (Binop op tar temp (Reg (temp+1))))))) ∧
   (inst_select_exp c tar temp (Shift sh exp nexp) =
-    let prog = inst_select_exp c temp temp exp in
-    (*nexp should be evaluated at compile time*) 
-    let n = num_exp nexp in 
-    Seq prog (Inst (Arith (Shift sh tar temp n)))) ∧ 
+    let n = num_exp nexp in
+    if (n < dimindex(:'a)) then
+      let prog = inst_select_exp c temp temp exp in
+      if n = 0 then
+        Seq prog (Move 0 [tar,temp])
+      else
+        Seq prog (Inst (Arith (Shift sh tar temp n)))
+    else
+      Inst (Const tar 0w)) ∧
   (*Make it total*)
   (inst_select_exp _ _ _ _ = Skip)`
   (WF_REL_TAC `measure (exp_size ARB o SND o SND o SND)`
@@ -121,18 +126,18 @@ EVAL ``inst_select_exp x64_config 0 99 (Op And [Const 99w;Op Add [Var 2;Var 3]])
 
 (*Flattens all expressions in program, temp must a fresh var*)
 val inst_select_def = Define`
-  (inst_select c temp (Assign v exp) = 
-    (inst_select_exp c v temp o flatten_exp) exp) ∧ 
+  (inst_select c temp (Assign v exp) =
+    (inst_select_exp c v temp o flatten_exp) exp) ∧
   (inst_select c temp (Set store exp) =
     let prog = (inst_select_exp c temp temp o flatten_exp) exp in
     Seq prog (Set store (Var temp))) ∧
   (inst_select c temp (Store exp var) =
     let exp = flatten_exp exp in
-    case exp of 
+    case exp of
     | Op Add [Const w;exp] =>
       let prog = inst_select_exp c temp temp exp in
-      if addr_offset_ok w c 
-      then 
+      if addr_offset_ok w c
+      then
         Seq prog (Inst (Mem Store var (Addr temp w)))
       else if c.valid_imm (INL Add) w
       then
@@ -144,27 +149,27 @@ val inst_select_def = Define`
         let prog'' = Inst (Arith (Binop Add temp temp (Reg (temp+1)))) in
         let prog''' = Inst (Mem Store var (Addr temp 0w)) in
         Seq prog (Seq prog' (Seq prog'' prog'''))
-        
-    | _ => 
+
+    | _ =>
       let prog = inst_select_exp c temp temp exp in
-        Seq prog (Inst (Mem Store var (Addr temp 0w)))) ∧ 
+        Seq prog (Inst (Mem Store var (Addr temp 0w)))) ∧
   (inst_select c temp (Seq p1 p2) =
-    Seq (inst_select c temp p1) (inst_select c temp p2)) ∧ 
+    Seq (inst_select c temp p1) (inst_select c temp p2)) ∧
   (inst_select c temp (If cmp r1 ri c1 c2) =
-    If cmp r1 ri (inst_select c temp c1) (inst_select c temp c2)) ∧ 
+    If cmp r1 ri (inst_select c temp c1) (inst_select c temp c2)) ∧
   (inst_select c temp (Call ret dest args handler) =
     let retsel =
-      case ret of 
+      case ret of
         NONE => NONE
       | SOME (n,names,ret_handler,l1,l2) =>
         SOME (n,names,inst_select c temp ret_handler,l1,l2) in
-    let handlersel = 
+    let handlersel =
       case handler of
         NONE => NONE
       | SOME (n,h,l1,l2) => SOME (n,inst_select c temp h,l1,l2) in
-    Call retsel dest args handlersel) ∧ 
+    Call retsel dest args handlersel) ∧
   (inst_select c temp prog = prog)`
-  
+
 (*
   Convert all 3 register instructions to 2 register instructions
 *)
@@ -172,22 +177,22 @@ val three_to_two_reg_def = Define`
   (three_to_two_reg (Inst (Arith (Binop bop r1 r2 ri))) =
     Seq (Move 0 [r1,r2]) (Inst (Arith (Binop bop r1 r1 ri)))) ∧
   (three_to_two_reg (Inst (Arith (Shift l r1 r2 n))) =
-    Seq (Move 0 [r1,r2]) (Inst (Arith (Shift l r1 r1 n)))) ∧ 
+    Seq (Move 0 [r1,r2]) (Inst (Arith (Shift l r1 r1 n)))) ∧
   (three_to_two_reg (Seq p1 p2) =
-    Seq (three_to_two_reg p1) (three_to_two_reg p2)) ∧ 
+    Seq (three_to_two_reg p1) (three_to_two_reg p2)) ∧
   (three_to_two_reg (If cmp r1 ri c1 c2) =
-    If cmp r1 ri (three_to_two_reg c1) (three_to_two_reg c2)) ∧ 
+    If cmp r1 ri (three_to_two_reg c1) (three_to_two_reg c2)) ∧
   (three_to_two_reg (Call ret dest args handler) =
     let retsel =
-      case ret of 
+      case ret of
         NONE => NONE
       | SOME (n,names,ret_handler,l1,l2) =>
         SOME (n,names,three_to_two_reg ret_handler,l1,l2) in
-    let handlersel = 
+    let handlersel =
       case handler of
         NONE => NONE
       | SOME (n,h,l1,l2) => SOME (n,three_to_two_reg h,l1,l2) in
-    Call retsel dest args handlersel) ∧ 
+    Call retsel dest args handlersel) ∧
   (three_to_two_reg prog = prog)`
 
 val _ = export_theory();
